verif/btrees.v
@@ -1,0 +1,424 @@
+(** * btrees.v : Formal Model of BTrees  *)
+
+Require Import VST.floyd.proofauto.
+Require Import VST.floyd.library.
+Require Import relation_mem.
+Instance CompSpecs : compspecs. make_compspecs prog. Defined.
+Definition Vprog : varspecs. mk_varspecs prog. Defined.
+
+Require Import VST.msl.wand_frame.
+Require Import VST.msl.iter_sepcon.
+Require Import VST.floyd.reassoc_seq.
+Require Import VST.floyd.field_at_wand.
+Require Import FunInd.
+
+(**
+    BTREES FORMAL MODEL
+ **)
+
+Definition Fanout := 15%nat.
+Lemma Fanout_eq : Fanout = 15%nat.
+Proof. reflexivity. Qed.
+Definition MaxTreeDepth := 20%nat.
+Lemma MTD_eq : MaxTreeDepth = 20%nat.
+Proof. reflexivity. Qed.
+
+Hint Rewrite Fanout_eq : rep_omega.
+Hint Rewrite MTD_eq : rep_omega.
+Global Opaque Fanout.
+Global Opaque MaxTreeDepth.
+
+Definition key := Z.            (* unsigned long in C *)
+Definition V:Type := Z.         (* I need some type for value_rep *)
+Variable b : nat.
+Variable X:Type.                (* val or unit *)
+
+Inductive entry (X:Type): Type :=
+     | keyval: key -> V -> X -> entry X
+     | keychild: key -> node X -> entry X
+with node (X:Type): Type :=
+     | btnode: option (node X) -> listentry X -> bool -> X -> node X
+with listentry (X:Type): Type :=
+     | nil: listentry X
+     | cons: entry X -> listentry X -> listentry X.
+
+Inductive index: Type :=
+| im: index
+| ip: nat -> index.
+
+Definition nat_to_index (n:nat) := ip n.
+
+Definition cursor (X:Type): Type := list (node X * index). (* ancestors and index *)
+Definition full_cursor (X:Type) : Type := bool * cursor X.
+Definition relation (X:Type): Type := node X * nat * X.  (* root and numRecords *)
+
+Definition next_index (i:index) : index :=
+  match i with
+  | im => ip (O%nat)
+  | ip n => ip (S n)
+  end.
+
+Fixpoint max_nat (m : nat) (n : nat) : nat :=
+  match m with
+  | O => n
+  | S m' => (match n with
+             | O => m
+             | S n' => S (max_nat m' n')
+             end)
+  end.
+
+Lemma max_0: forall a, max_nat a 0 = a.
+Proof. induction a. auto. simpl. auto. Qed.
+
+Theorem le_max_split_l: forall n a b,
+    (n < a)%nat -> (n< max_nat a b)%nat.
+Proof.
+  intros.
+  generalize dependent n.
+  generalize dependent b0.
+  generalize dependent a.
+  induction a; intros.
+  - inversion H.
+  - destruct b0.
+    + rewrite max_0. auto.
+    + simpl. destruct n. omega.
+      assert (n<a)%nat by omega. apply IHa with (b0:=b0) in H0. omega.
+Qed.      
+
+Theorem max_flip: forall a b, max_nat a b = max_nat b a.
+Proof.
+  induction a; intros.
+  - simpl. rewrite max_0. auto.
+  - simpl. destruct b0.
+    + simpl. auto.
+    + simpl. rewrite IHa. auto.
+Qed.    
+
+Theorem le_max_split_r: forall n a b,
+    (n < b)%nat -> (n< max_nat a b)%nat.
+Proof.
+  intros. rewrite max_flip. apply le_max_split_l. auto.
+Qed.
+  
+Definition max_index (i1:index) (i2:index): index :=
+  match i1 with
+  | im => i2
+  | ip n1 => match i2 with
+            | im => i1
+            | ip n2 => ip (max_nat n1 n2)
+             end
+  end.
+
+Fixpoint node_depth {X:Type} (n:node X) : nat :=
+  match n with
+    btnode ptr0 le _ _ => max_nat (listentry_depth le)
+                                (match ptr0 with
+                                 | None => O
+                                 | Some n' => S (node_depth n') end)
+  end
+with listentry_depth {X:Type} (le:listentry X) : nat :=
+       match le with
+       | nil => O
+       | cons e le' => max_nat (entry_depth e) (listentry_depth le')
+       end
+with entry_depth {X:Type} (e:entry X) : nat :=
+       match e with
+       | keyval _ _ _ => S O
+       | keychild _ n => S (node_depth n)
+       end.                                                 
+
+Fixpoint nth_entry_le {X:Type} (i:nat) (le:listentry X): option (entry X) :=
+  match i with
+  | O => match le with
+         | nil => None
+         | cons e _ => Some e
+         end
+  | S i' => match le with
+            | nil => None
+            | cons _ le' => nth_entry_le i' le'
+            end
+  end.                          (* USEFUL? *)
+
+Fixpoint numKeys_le {X:Type} (le:listentry X) : nat :=
+  match le with
+  | nil => 0%nat
+  | cons e le' => S (numKeys_le le')
+  end.
+
+Definition numKeys {X:Type} (n:node X) : nat :=
+  match n with btnode ptr0 le _ x => numKeys_le le end.
+
+  
+Fixpoint move_to_first {X:Type} (c:cursor X) (curr:node X): cursor X:=
+  match curr with btnode ptr0 le _ _ =>
+                  match ptr0 with
+                  | Some n => move_to_first ((curr,im)::c) n
+                  | None => match le with
+                            | nil => c (* possible? *)
+                            | cons e le' => match e with
+                                            | keyval _ _ _ => ((curr,ip (0%nat))::c)
+                                            | keychild _ _ => c (* not possible, we would have a ptr0 otherwise *)
+                                            end
+                            end
+                  end
+  end.
+
+Fixpoint full_move_to_first {X:Type} (csr:full_cursor X) (curr:node X): full_cursor X:=
+  match csr with (b,c) =>
+                 match numKeys curr with
+                                    | O => (false, move_to_first c curr)
+                                    | _ => (true, move_to_first c curr)
+                 end
+  end.
+
+Fixpoint le_length {X:Type} (le:listentry X) : nat :=
+  match le with
+  | nil => O
+  | cons _ le' => S (le_length le')
+  end.
+
+Definition node_length {X:Type} (n:node X) : nat :=
+  match n with btnode ptr0 le _ _ => le_length le end.
+
+Definition index_leb_nat (i:index) (n:nat) : bool :=
+  match i with
+  | im => true
+  | ip n' => (n' <=? n)%nat
+  end.
+
+Fixpoint move_to_next_partial {X:Type} (c:cursor X) : cursor X :=
+  match c with
+  | [] => []
+  | (n,i)::c' =>
+    match (index_leb_nat i (node_length n -2)) with 
+    | true => (n,next_index i)::c'
+    | false => move_to_next_partial c'
+    end
+  end.
+
+Fixpoint nth_node_le {X:Type} (i:nat) (le:listentry X): option (node X) :=
+  match i with
+  | O => match le with
+         | nil => None
+         | cons e _ => match e with
+                       | keychild _ n => Some n
+                       | keyval _ _ _ => None
+                       end
+         end
+  | S i' => match le with
+            | nil => None
+            | cons _ le' => nth_node_le i' le'
+            end
+  end.
+
+Lemma nth_node_le_decrease: forall X (le:listentry X) (n:node X) i,
+    nth_node_le i le = Some n ->
+    (node_depth n < listentry_depth le)%nat.
+Proof.
+  induction le; intros.
+  - unfold nth_node_le in H.
+    destruct i; inversion H.
+  - simpl.
+    destruct i.
+    + apply le_max_split_l. simpl in H. destruct e; try inv H. simpl. auto.
+    + apply le_max_split_r. apply IHle with (i:=i). simpl in H. auto.
+Qed.
+      
+Definition nth_node {X:Type} (i:index) (n:node X): option (node X) :=
+  match n with btnode ptr0 le _ _ =>
+               match i with
+               | im => ptr0
+               | ip na => nth_node_le na le
+               end
+  end.
+
+Lemma nth_node_decrease: forall X (n:node X) (n':node X) i,
+    nth_node i n = Some n' ->
+    (node_depth n' < node_depth n)%nat.
+Proof.
+  intros. unfold nth_node in H.
+  destruct n. destruct i.
+  - simpl. destruct o. inversion H. subst.
+    apply le_max_split_r. auto. inversion H.
+  - simpl. apply le_max_split_l. apply nth_node_le_decrease with (i:=n). auto.
+Qed.
+
+Definition move_to_next {X:Type} (c:cursor X): cursor X * bool :=
+  match (move_to_next_partial c) with
+  | [] => (c,false)                     (* C program returns false here *)
+  | (n,i)::c' => match nth_node i n with
+                 | Some n' => (move_to_first c n',true)
+                 | None => (c,true)    (* possible at leaf nodes *)
+                 end
+  end.
+
+Definition getRecord (c:cursor val): val :=
+  match c with
+  | [] => nullval
+  | (n,i)::c' =>
+    match n with
+      btnode ptr0 le b x =>
+      match i with
+      | im => nullval              (* no -1 at leaf nodes *)
+      | ip ii =>
+        match (nth_entry_le ii le) with
+        | None => nullval
+        | Some e =>
+          match e with
+          | keychild _ _ => nullval
+          | keyval k v x => x
+          end
+        end
+      end
+    end
+  end.
+
+Definition getKey {X:Type} (c:cursor X): option key :=
+  match c with
+  | [] => None
+  | (n,i)::c' =>
+    match n with
+      btnode ptr0 le b x =>
+      match i with
+      | im => None            (* ptr0 has no key *)
+      | ip ii => 
+        match (nth_entry_le ii le) with
+        | None => None
+        | Some e =>
+          match e with
+          | keychild k _ => Some k
+          | keyval k _ _ => Some k
+          end
+        end
+      end
+    end
+  end.
+
+Fixpoint findChildIndex' {X:Type} (le:listentry X) (key:key) (i:index): index :=
+  match le with
+  | nil => i
+  | cons e le' =>
+    match e with
+    | keyval k v x =>
+      match (key <=? k) with
+      | true => i
+      | false => findChildIndex' le' key (next_index i)
+      end
+    | keychild k c =>
+      match (key <=? k) with
+      | true => i
+      | false => findChildIndex' le' key (next_index i)
+      end
+    end
+  end.
+
+Definition findChildIndex {X:Type} (le:listentry X) (key:key): index :=
+  findChildIndex' le key im.
+
+(* n should be the current node pointed to, so if c=(m,i)::c', it should be m(i) *)
+Function moveToRecord {X:Type} (c:cursor X) (key:key) (n:node X) {measure node_depth n}: cursor X * bool :=
+  match n with btnode ptr0 le isLeaf x =>
+               match isLeaf with
+               | true =>
+                 match findChildIndex le key with
+                 | im => ((n,ip 0)::c, false)
+                 | ip ii =>
+                   match getKey ((n,ip ii)::c) with
+                   | None => (c,false)  (* shouldnt happen, findChildIndex return valid indexes *)
+                   | Some k => ((n,ip ii)::c, key =? k)
+                   end
+                 end
+               | false =>
+                 match nth_node (findChildIndex le key) n with
+                 | None => (c,false)    (* should not happen: we should have ptr0 and findChildIndex should not overflow *)
+                 | Some n' =>
+                   moveToRecord ((n,findChildIndex le key)::c) key n'
+                 end
+               end
+  end.
+Proof.
+  intros.
+  apply nth_node_decrease with (i:= findChildIndex le key0). auto.
+Qed.
+
+Fixpoint update_le_nth_child {X:Type} (i:nat) (le:listentry X) (n:node X) : listentry X :=
+  match le with
+  | nil => nil X
+  | cons e le' => match i with
+                  | O => match e with
+                         | keychild k c => cons X (keychild X k n) le'
+                         | keyval k v x => cons X (keychild X k n) le' (* shouldnt happen *)
+                         end
+                  | S i' => update_le_nth_child i' le' n
+                  end
+  end.  
+
+Fixpoint update_le_nth_val {X:Type} (i:nat) (le:listentry X) (newv:V) (newx:X) : listentry X :=
+  match le with
+  | nil => nil X
+  | cons e le' => match i with
+                  | O => match e with
+                         | keychild k c => cons X (keyval X k newv newx) le' (* shouldnt happen *)
+                         | keyval k v x => cons X (keyval X k newv newx) le'
+                         end
+                  | S i' => update_le_nth_val i' le' newv newx
+                  end
+  end.
+
+Definition update_node_nth_child {X:Type} (i:index) (oldn:node X) (n:node X) : node X :=
+  match oldn with btnode ptr0 le isLeaf x =>
+  match i with
+  | im => btnode X (Some n) le isLeaf x
+  | ip ii => btnode X ptr0 (update_le_nth_child ii le n) isLeaf x
+  end
+  end.
+
+Fixpoint update_cursor {X:Type} (c:cursor X) (n:node X) : cursor X :=
+  match c with
+  | [] => []
+  | (oldn,i)::c' =>
+    let newn := update_node_nth_child i oldn n in
+    (newn,i)::(update_cursor c' newn)
+  end.
+
+Fixpoint nth_key {X:Type} (i:nat) (le:listentry X): option key :=
+  match le with
+  | nil => None
+  | cons e le' => match i with
+                  | O => match e with
+                         | keychild k _ => Some k
+                         | keyval k _ _ => Some k
+                         end
+                  | S i' => nth_key i' le'
+                  end
+  end.
+  
+(* c should not be complete, and points to n *)
+(* nEFC is newEntryFromChild pointer *)
+Fixpoint insertKeyRecord' {X:Type} (key:key) (value:V) (nEFC:X) (n:node X) (c:cursor X): node X * cursor X * bool :=
+  match n with btnode ptr0 le isLeaf x =>
+  match isLeaf with
+  | true =>
+    match le with
+    | nil =>               (* first key *)
+      let newn:= btnode X ptr0 (cons X (keyval X key value nEFC) (nil X)) isLeaf x in
+      (newn,update_cursor c newn,true)
+    | _ =>
+      match (findChildIndex le key) with
+      | im => (n,c,false) (* TODO: THIS IS NOT ADDRESSED IN THE C CODE!!! *)
+      | ip ii =>
+        match (nth_key ii le) with
+        | None => (n,c,false)   (* impossible, findChildIndex returns an index in range ? *)
+        | Some k =>
+          match (k =? key) with
+          | true =>             (* update *)
+            let newn:= btnode X ptr0 (update_le_nth_val ii le value nEFC) isLeaf x in
+            (newn,update_cursor c newn,true) (* I don't think we should use nEFC. wich val? *)
+          | false => (n,c,false)          (* new node, TODO *)
+          end
+        end
+      end
+    end
+  | false => (n,c,false) (* TODO *)
+  end
+  end.
