verif/btrees_sep.v
@@ -1,0 +1,280 @@
+(** * btrees_sep.v : Representation omf btrees in Separation Logic *)
+
+Require Import VST.floyd.proofauto.
+Require Import VST.floyd.library.
+Require Import relation_mem.
+Instance CompSpecs : compspecs. make_compspecs prog. Defined.
+Definition Vprog : varspecs. mk_varspecs prog. Defined.
+
+Require Import VST.msl.wand_frame.
+Require Import VST.msl.iter_sepcon.
+Require Import VST.floyd.reassoc_seq.
+Require Import VST.floyd.field_at_wand.
+Require Import FunInd.
+Require Import btrees.
+
+(**
+    REPRESENTATIONS IN SEPARATION LOGIC
+ **)
+
+Definition tbtnode:=      Tstruct _BtNode noattr.
+Definition tentry:=       Tstruct _Entry noattr.
+Definition tchildrecord:= Tunion _Child_or_Record noattr.
+Definition trelation:=    Tstruct _Relation noattr.
+Definition tcursor:=      Tstruct _Cursor noattr.
+
+Definition value_rep (v:V) (p:val):= (* this should change if we change the type of Values? *)
+  data_at Tsh tint (Vint (Int.repr v)) p.
+
+Definition isLeaf {X:Type} (n:node X) : bool :=
+  match n with btnode ptr0 le b w => b end.
+
+Definition getval (n:node val): val :=
+  match n with btnode _ _ _ x => x end.
+
+Fixpoint le_to_list (le:listentry val) : list (val * (val + val)) :=
+  match le with
+  | nil => []
+  | cons e le' =>
+    (match e with
+     | keychild k c => ((Vlong(Int64.repr k)),  inl (getval c))
+     | keyval k v x => ((Vlong(Int64.repr k)),  inr x) (* ptr to the record?? *)
+     end) :: le_to_list le'
+  end.
+
+Definition le_to_list_complete (le:listentry val):=
+  le_to_list le ++ list_repeat (Fanout - numKeys_le le) (Vundef, inl Vundef).
+                        
+Fixpoint entry_rep (e:entry val):=
+  match e with
+  | keychild _ n => match n with btnode _ _ _ x => btnode_rep n x end
+  | keyval _ v x => value_rep v x
+  end
+with btnode_rep (n:node val) (p:val):mpred :=
+  match n with btnode ptr0 le b x =>
+  !!(x=p) &&
+  malloc_token Tsh tbtnode p *
+  field_at Tsh tbtnode (DOT _numKeys) (Vint(Int.repr (Z.of_nat (numKeys n)))) p *
+  field_at Tsh tbtnode (DOT _isLeaf) (Val.of_bool b) p *
+  match ptr0 with
+  | None => field_at Tsh tbtnode (DOT _ptr0) nullval p
+  | Some n' => match n' with btnode _ _ _ p' => field_at Tsh tbtnode (DOT _ptr0) p' p * btnode_rep n' p' end
+  end *
+  field_at Tsh tbtnode (DOT _entries) (le_to_list_complete le) p *
+  le_iter_sepcon le
+  end
+with le_iter_sepcon (le:listentry val):mpred :=
+  match le with
+  | nil => emp
+  | cons e le' => entry_rep e * le_iter_sepcon le'
+  end.
+
+Definition get_val (n:node val) : val :=
+  match n with btnode _ _ _ x => x end.
+
+Lemma btnode_rep_local_prop: forall n p,
+    btnode_rep n p |-- !!(isptr p).
+Proof.
+  intros. destruct n. unfold btnode_rep. Intros. subst. entailer!.
+Qed.
+
+Lemma btnode_rep_local_prop2: forall n p,
+    btnode_rep n p |-- !!(p = get_val n).
+Proof.
+  intros. destruct n. unfold btnode_rep. Intros. subst. entailer!.
+Qed.
+  
+Hint Resolve btnode_rep_local_prop: saturate_local.
+Hint Resolve btnode_rep_local_prop2: saturate_local.
+
+Lemma btnode_valid_pointer: forall n p,
+    btnode_rep n p |-- valid_pointer p.
+Proof.
+  intros. destruct n. unfold btnode_rep. entailer!.
+Qed.
+
+Hint Resolve btnode_valid_pointer: valid_pointer.
+
+Definition relation_rep (r:relation val) (p:val):mpred :=
+  match r with
+  | (n,c,x) => !!(x=p) &&
+    EX p':val,
+          field_at Tsh trelation (DOT _root) p' p *
+          btnode_rep n p' *
+          field_at Tsh trelation (DOT _numRecords) (Vlong(Int64.repr(Z.of_nat c))) p * (* long?int? *)
+          malloc_token Tsh trelation p
+  end.
+
+Lemma relation_rep_local_prop: forall r p,
+    relation_rep r p |-- !!(isptr p).
+Proof. 
+  intros. destruct r. unfold relation_rep. destruct p0. Intros p'. entailer!.
+Qed.
+
+Lemma relation_rep_local_prop2: forall r p,
+    relation_rep r p |-- !!(p = snd r).
+Proof. 
+  intros. destruct r. unfold relation_rep. destruct p0. Intros p'. entailer!.
+Qed.
+
+Hint Resolve relation_rep_local_prop: saturate_local.
+Hint Resolve relation_rep_local_prop2: saturate_local.
+
+Lemma relation_rep_valid_pointer: forall r p,
+    relation_rep r p |-- valid_pointer p.
+Proof.
+  intros. destruct r. unfold relation_rep. destruct p0. Intros p'. entailer!.
+Qed.
+
+Hint Resolve relation_rep_valid_pointer: valid_pointer.
+  
+Definition getCurrVal (c:cursor val): val :=
+  match c with
+  | [] => nullval
+  | (n,_)::_ => match n with btnode _ _ _ x => x end
+  end.
+
+Definition getEntryIndex {X:Type} (c:cursor X) : index :=
+  match c with
+  | (n,i)::_ => i
+  | [] => ip (0%nat)
+  end.
+
+Fixpoint cursor_valid_bool {X:Type} (c:cursor X): bool :=
+  match c with
+  | [] => true
+  | (b,i)::c' => match b with btnode ptr0 le _ x => (index_leb_nat i (numKeys_le le -1)) && cursor_valid_bool c' end
+  end.                          (* might be incomplete *)
+
+Definition rep_index (i:index):=
+  match i with
+  | im => Vint(Int.repr(-1))
+  | ip n => Vint(Int.repr(Z.of_nat n))
+  end.
+
+Definition cursor_rep (c:cursor val) (r:relation val) (p:val):mpred :=
+  EX anc_end:list val, EX idx_end:list val,
+  malloc_token Tsh tcursor p *
+  field_at Tsh tcursor (DOT _currNode) (getCurrVal c) p *
+  match r with (n,c,x) => field_at Tsh tcursor (DOT _relation) x p end *
+  field_at Tsh tcursor (DOT _entryIndex) (rep_index(getEntryIndex c)) p *
+  field_at Tsh tcursor (DOT _isValid) (Val.of_bool (cursor_valid_bool c)) p *
+  field_at Tsh tcursor (DOT _level) (Vint(Int.repr(Zlength c))) p *
+  field_at Tsh tcursor (DOT _nextAncestorPointerIdx) ((map (fun x => (rep_index (snd x)))  c) ++ idx_end) p * (* or its reverse? *)
+  field_at Tsh tcursor (DOT _ancestors) ((map getval (map fst c)) ++ anc_end) p.
+
+Lemma cursor_rep_local_prop: forall c r p,
+    cursor_rep c r p |-- !!(isptr p).
+Proof. 
+  intros. unfold cursor_rep. Intros a. Intros i. entailer!.
+Qed.
+
+Hint Resolve cursor_rep_local_prop: saturate_local.
+
+Lemma cursor_rep_valid_pointer: forall c r p,
+    cursor_rep c r p |-- valid_pointer p.
+Proof.
+  intros. unfold cursor_rep. Intros a. Intros i. entailer!.
+Qed.    
+
+Hint Resolve cursor_rep_valid_pointer: valid_pointer.
+
+Inductive subnode {X:Type} : node X -> node X -> Prop :=
+| sub_refl: forall n, subnode n n
+| sub_ptr0: forall n le b x, subnode n (btnode X (Some n) le b x)
+| sub_entr: forall n p le b x k, subnode n (btnode X p (cons X (keychild X k n) le) b x)
+| sub_cons: forall n p le e b x, subnode n (btnode X p le b x) ->
+                                 subnode n (btnode X p (cons X e le) b x)
+| sub_trans: forall n n1 n2, subnode n n1 -> subnode n1 n2 -> subnode n n2.
+
+
+Lemma btnode_rep_simpl_ptr0: forall le b x (p0:option (node val)) le0 b0 x0 proot p0,
+    btnode_rep (btnode val (Some (btnode val p0 le0 b0 x0)) le b x) proot =
+    !!(x=proot) &&
+      malloc_token Tsh tbtnode proot *
+    field_at Tsh tbtnode (DOT _numKeys) (Vint(Int.repr (Z.of_nat (numKeys_le le)))) proot *
+    field_at Tsh tbtnode (DOT _isLeaf) (Val.of_bool b) proot *
+    field_at Tsh tbtnode (DOT _ptr0) x0 proot *
+    btnode_rep (btnode val p0 le0 b0 x0) x0 *
+    field_at Tsh tbtnode (DOT _entries) (le_to_list_complete le) proot *
+    le_iter_sepcon le.
+Proof.
+  intros. apply pred_ext; entailer!; simpl; entailer!.
+Qed.
+
+Lemma btnode_rep_simpl_keychild: forall ptr0 le b x proot k nptr0 nle nb nx,
+    btnode_rep (btnode val ptr0 (cons val (keychild val k (btnode val nptr0 nle nb nx)) le) b x) proot =
+    !!(x=proot) &&
+      malloc_token Tsh tbtnode proot *
+    field_at Tsh tbtnode (DOT _numKeys) (Vint(Int.repr (Z.of_nat (S (numKeys_le le))))) proot *
+    field_at Tsh tbtnode (DOT _isLeaf) (Val.of_bool b) proot *
+    match ptr0 with
+    | None => field_at Tsh tbtnode (DOT _ptr0) nullval proot
+    | Some n' => match n' with btnode _ _ _ p' => field_at Tsh tbtnode (DOT _ptr0) p' proot * btnode_rep n' p' end
+    end *
+    field_at Tsh tbtnode (DOT _entries) (le_to_list_complete (cons val (keychild val k (btnode val nptr0 nle nb nx)) le)) proot *
+    btnode_rep (btnode val nptr0 nle nb nx) nx *
+    le_iter_sepcon le.
+Proof.
+  intros. apply pred_ext; entailer!; simpl; entailer!.
+Qed.
+
+Theorem subnode_rep: forall n root proot,
+    subnode n root ->
+    btnode_rep root proot |-- EX pn:val, btnode_rep n pn *
+                              (btnode_rep n pn -* btnode_rep root proot).
+Proof.
+  intros.
+  induction H.
+  - Exists proot. cancel. rewrite <- wand_sepcon_adjoint. cancel.
+  - destruct n. Exists v. rewrite btnode_rep_simpl_ptr0 by auto.
+    entailer!. rewrite <- wand_sepcon_adjoint. entailer!.
+  - destruct n. Exists v. rewrite btnode_rep_simpl_keychild.
+    entailer!. rewrite <- wand_sepcon_adjoint. entailer!.
+  - admit.                      (* we can't use the induction hypothesis *)
+  - admit.                      (* same *)
+Admitted.
+
+Fixpoint cursor_correct {X:Type} (c:cursor X) (n:node X) (root:node X): Prop :=
+  match c with
+  | [] => n = root
+  | (n',i)::c' => (cursor_correct c' n' root) /\ (nth_node i n' = Some n)
+  end.
+
+Definition get_root {X:Type} (rel:relation X) : node X := fst (fst rel).
+
+Definition cursor_correct_rel {X:Type} (c:cursor X) (rel:relation X): Prop :=
+  match c with
+  | [] => True
+  | (n,i)::c' => match nth_node i n with
+                 | None => False
+                 | Some n' => cursor_correct c n' (get_root rel)
+                 end
+  end.
+
+Lemma nth_subnode: forall X i (n:node X) n',
+    nth_node i n' = Some n -> subnode n n'.
+Proof.
+  intros.
+  induction i.
+  - unfold nth_node in H. destruct n'. subst. apply sub_ptr0.
+  - destruct n' as [ptr0 le isLeaf x]. simpl in H.
+    generalize dependent n. generalize dependent le. induction n0.
+    + intros. destruct le; simpl in H. inv H. destruct e; inv H.
+      apply sub_entr.
+    + intros. simpl in H. destruct le. inv H.
+      apply IHn0 in H. apply sub_cons. auto.
+Qed.
+
+Theorem cursor_subnode: forall X (c:cursor X) root n,
+    cursor_correct c n root ->
+    subnode n root.
+Proof.
+  intros. generalize dependent n.
+  induction c.
+  - intros. simpl in H. subst. apply sub_refl.
+  - intros. destruct a as [n' i]. simpl in H.
+    destruct H. apply IHc in H. apply nth_subnode in H0.
+    eapply sub_trans; eauto.
+Qed.
+
