verif/btrees_spec.v
@@ -1,0 +1,84 @@
+(** * btrees_spec.v : Specifications of relation_mem.c functions *)
+
+Require Import VST.floyd.proofauto.
+Require Import VST.floyd.library.
+Require Import relation_mem.
+Instance CompSpecs : compspecs. make_compspecs prog. Defined.
+Definition Vprog : varspecs. mk_varspecs prog. Defined.
+
+Require Import VST.msl.wand_frame.
+Require Import VST.msl.iter_sepcon.
+Require Import VST.floyd.reassoc_seq.
+Require Import VST.floyd.field_at_wand.
+Require Import FunInd.
+Require Import btrees.
+Require Import btrees_sep.
+
+(**
+    FUNCTION SPECIFICATIONS
+ **)
+Definition empty_node (b:bool) (p:val):node val := (btnode val) None (nil val) b p.
+Definition empty_relation (pr:val) (pn:val): relation val := ((empty_node true pn),0%nat,pr).
+Definition empty_cursor := []:cursor val.
+
+Definition createNewNode_spec : ident * funspec :=
+  DECLARE _createNewNode
+  WITH isLeaf:bool
+  PRE [ _isLeaf OF tint ]       (* why tint and not tbool? *)
+  PROP ()
+  LOCAL (temp _isLeaf (Val.of_bool isLeaf))
+  SEP ()
+  POST [ tptr tbtnode ]
+  EX p:val, PROP ()
+  LOCAL (temp ret_temp p)
+  SEP (if (eq_dec p nullval) then emp else btnode_rep (empty_node isLeaf p) p).
+(* not strong enough? *)
+
+Definition RL_NewRelation_spec : ident * funspec :=
+  DECLARE _RL_NewRelation
+  WITH u:unit
+  PRE [ ]
+  PROP ()
+  LOCAL ()
+  SEP ()
+  POST [ tptr trelation ]
+  EX pr:val, EX pn:val, PROP ()
+  LOCAL(temp ret_temp pr)
+  SEP (if (eq_dec pr nullval) then emp else relation_rep (empty_relation pr pn) pr).
+
+Definition RL_NewCursor_spec : ident * funspec :=
+  DECLARE _RL_NewCursor
+  WITH r:relation val, p:val
+  PRE [ _relation OF tptr trelation ]
+  PROP ()
+  LOCAL (temp _relation p)
+  SEP (relation_rep r p)
+  POST [ tptr tcursor ]
+  EX p':val, PROP ()
+  LOCAL(temp ret_temp p')
+  SEP (relation_rep r p * (if (eq_dec p' nullval)
+                           then emp
+                           else cursor_rep empty_cursor r p')).
+
+Definition RL_MoveToNext_spec : ident * funspec :=
+  DECLARE _RL_MoveToNext
+  WITH c:cursor val, p:val, rel:relation val, prel:val
+  PRE [ _btCursor OF tptr tcursor ]
+  PROP (cursor_correct_rel c rel)
+  LOCAL (temp _btCursor p)
+  SEP (cursor_rep c rel p; relation_rep rel prel)
+  POST [ tint ]
+  EX b:bool, EX c':cursor val,
+  PROP (move_to_next c = (c',b); cursor_correct_rel c' rel)
+  LOCAL (temp ret_temp (Val.of_bool b))
+  SEP(cursor_rep c' rel p; relation_rep rel prel).
+                             
+(**
+    GPROG
+ **)
+
+Definition Gprog : funspecs :=
+        ltac:(with_library prog [
+                             createNewNode_spec; RL_NewRelation_spec; RL_NewCursor_spec;
+                             RL_MoveToNext_spec
+ ]).
