verif/verif_newcursor.v
@@ -1,0 +1,101 @@
+(** * verif_newcursor.v: Correctness proof of newCursor *)
+
+Require Import VST.floyd.proofauto.
+Require Import VST.floyd.library.
+Require Import relation_mem.
+Instance CompSpecs : compspecs. make_compspecs prog. Defined.
+Definition Vprog : varspecs. mk_varspecs prog. Defined.
+
+Require Import VST.msl.wand_frame.
+Require Import VST.msl.iter_sepcon.
+Require Import VST.floyd.reassoc_seq.
+Require Import VST.floyd.field_at_wand.
+Require Import FunInd.
+Require Import btrees.
+Require Import btrees_sep.
+Require Import btrees_spec.
+
+Lemma upd_repeat: forall X i (a:X) b m, 0 <= i -> (Z.to_nat i <= m)%nat -> m=MaxTreeDepth ->  
+    upd_Znth i (list_repeat (Z.to_nat i) a ++ list_repeat (m - Z.to_nat i) b) a =
+    (list_repeat (Z.to_nat (i+1)) a) ++ list_repeat (m - Z.to_nat (i+1)) b.
+Proof.
+  intros. assert (Z.to_nat (i + 1) = ((Z.to_nat i) + S O)%nat).
+  rewrite Z2Nat.inj_add; auto. omega.
+  rewrite H2.
+  rewrite <- list_repeat_app.
+  rewrite upd_Znth_app2. 
+  rewrite Zlength_list_repeat by auto.
+  simpl. assert (i-i=0). omega. rewrite H3.
+  unfold upd_Znth. simpl.
+  assert ((m - (Z.to_nat i))%nat = Z.to_nat (20-i)).
+  admit. rewrite H4.
+  rewrite sublist_list_repeat.
+  admit.
+  omega. admit.                  (* false! *)
+  rewrite Zlength_list_repeat. split. omega. admit. auto.  
+Admitted.
+
+Lemma body_NewCursor: semax_body Vprog Gprog f_RL_NewCursor RL_NewCursor_spec.
+Proof.
+  start_function.
+forward_if (PROP() LOCAL(temp _relation p) SEP(relation_rep r p))%assert.
+- forward. auto.
+- subst p.
+  (* forward_call tt. *)              (* telling me to import VST.floyd.library, but it has been done *)
+  admit.
+- forward_call tcursor.
+  + split. unfold sizeof. simpl. rep_omega. split; auto.
+  + Intros vret.
+    forward_if ((PROP (vret<>nullval)
+     LOCAL (temp _cursor vret; temp _relation p)
+     SEP (if eq_dec vret nullval
+          then emp
+          else malloc_token Tsh tcursor vret * data_at_ Tsh tcursor vret; 
+          relation_rep r p))).
+    * if_tac; entailer!.
+    * rewrite if_true; auto.
+      forward. Exists nullval. entailer!.
+    * forward. rewrite if_false; auto. entailer!.
+    * Intros. rewrite if_false; auto. Intros.
+      forward.                  (* cursor->relation=relation *)
+      forward.                  (* cursor->currnode=null *)
+      forward.                  (* cursor->entryIndex=0 *)
+      forward.                  (* cursor->isValid=0 *)
+      forward.                  (* cursor->level=0 *)
+      autorewrite with norm. simpl.
+      pose (n:=20).
+      pose (Pre:=(EX i:Z,
+            PROP ((0 <= i)%Z; (i <= n)%Z)
+            LOCAL(temp _cursor vret; temp _relation p)         
+            SEP(malloc_token Tsh tcursor vret;
+                relation_rep r p;
+                data_at Tsh tcursor
+               (force_val (sem_cast_pointer p),
+               (Vint (Int.repr 0),
+               (Vint (Int.repr 0),
+               (Vint (Int.repr 0),
+               (Vint (Int.repr 0),
+               (list_repeat (Z.to_nat i) (Vint(Int.repr 0)) ++  list_repeat (MaxTreeDepth - (Z.to_nat i)) Vundef,
+                (list_repeat (Z.to_nat i) nullval ++ list_repeat (MaxTreeDepth - (Z.to_nat i)) Vundef))))))) vret))%assert).
+      { 
+        forward_for_simple_bound n Pre.
+        - autorewrite with sublist. entailer!.
+        - Intros.
+          forward.              (* cursor->nextancestorptridx[i]=0 *)
+          forward.              (* cursor->ancestors[i]=null *)
+          assert (MaxTreeDepth = Z.to_nat 20). rewrite MTD_eq. simpl. auto.
+          entailer!. rewrite upd_repeat. rewrite upd_repeat. entailer!.
+          auto. rewrite H3. apply Z2Nat.inj_le. auto. omega. auto.
+          auto. auto. rewrite H3. apply Z2Nat.inj_le. auto. omega. auto. auto.
+        - forward.              (* return *)
+          Exists vret. entailer!.
+          rewrite if_false by auto.
+          unfold cursor_rep.  Exists (list_repeat 20 nullval). Exists (list_repeat 20 (Vint(Int.repr 0))).
+          entailer!. autorewrite with sublist.
+          unfold_data_at 1%nat. simpl. entailer!.
+          rewrite field_at_data_at. entailer!.
+          destruct r. destruct p.
+          rewrite <- field_at_data_at. simpl. cancel. unfold Vtrue.
+          admit.                (* my isValid definition is wrong. add it to the cursor type? *)
+      } 
+Admitted.
