verif/verif_newrel.v
@@ -1,0 +1,59 @@
+(** * verif_newrel.v: Correctness proof of NewRelation *)
+
+Require Import VST.floyd.proofauto.
+Require Import VST.floyd.library.
+Require Import relation_mem.
+Instance CompSpecs : compspecs. make_compspecs prog. Defined.
+Definition Vprog : varspecs. mk_varspecs prog. Defined.
+
+Require Import VST.msl.wand_frame.
+Require Import VST.msl.iter_sepcon.
+Require Import VST.floyd.reassoc_seq.
+Require Import VST.floyd.field_at_wand.
+Require Import FunInd.
+Require Import btrees.
+Require Import btrees_sep.
+Require Import btrees_spec.
+
+Lemma body_NewRelation: semax_body Vprog Gprog f_RL_NewRelation RL_NewRelation_spec.
+Proof.
+start_function.
+forward_call(true).
+Intros vret.
+forward_if(PROP (vret<>nullval)
+     LOCAL (temp _pRootNode vret)
+     SEP (if eq_dec vret nullval then emp else btnode_rep (empty_node true vret) vret)).
+- if_tac; entailer!.
+- subst vret. forward. Exists nullval. Exists nullval. entailer!.
+- forward. rewrite if_false by auto. entailer!.
+- forward_call trelation.
+  + split. unfold sizeof. simpl. rep_omega. split; auto.
+  + Intros newrel.
+    forward_if(PROP (newrel<>nullval)
+     LOCAL (temp _pNewRelation newrel; temp _pRootNode vret)
+     SEP (if eq_dec newrel nullval
+          then emp
+          else malloc_token Tsh trelation newrel * data_at_ Tsh trelation newrel;
+          if eq_dec vret nullval then emp else btnode_rep (empty_node true vret) vret)).
+    * if_tac; entailer!.
+    * rewrite if_true by auto. rewrite if_false by auto. subst newrel.
+      forward_call (tbtnode, vret). (* free *)
+      { unfold btnode_rep. simpl. Intros. cancel.
+        unfold data_at_. unfold field_at_. simpl.
+        (* Frame should be empty *)
+        (* default val should be the way we instantiated it -> comes from free spec? *)
+       admit.
+      }
+      { forward.
+        Exists (Vint(Int.repr 0)). Exists vret. rewrite if_true by auto. entailer!.
+        admit. }
+    * rewrite if_false; auto.
+      forward.
+      entailer!. rewrite if_false; auto.
+    * Intros. rewrite if_false; auto. Intros.
+      forward.                  (* pnewrelation->root = prootnode *)
+      forward.                  (* pnewrelation->numrecords=0 *)
+      forward.                  (* return pnewrelation *)
+      Exists newrel. Exists vret. rewrite if_false by auto. rewrite if_false by auto. Exists vret.
+      entailer!. unfold_data_at 1%nat. cancel.
+Admitted.
